A decent formalization.

Casper.thy
@@ -1,67 +1,89 @@
 theory Casper
-imports Main
+imports Main "Eisbach"
 begin
 
 locale byz_quorums =
-  fixes member_1 :: "'n \<Rightarrow> 'q1 \<Rightarrow> bool" (* membership in 2/3 set *)
-    and member_2 :: "'n \<Rightarrow> 'q2 \<Rightarrow> bool" (* membership in 1/3 set *)
-  assumes "\<And> q1 q2 . \<exists> q3 . \<forall> n . member_2 n q3 \<longrightarrow> member_1 n q1 \<and> member_1 n q2" (* 2/3 quorums have 1/3 intersection *)
-    and "\<And> q1 q2 . \<exists> n . member_2 n q1 \<and> member_1 n q2" (* 2/3 sets and 1/3 sets intersect *)
+  fixes member_1 :: "'n \<Rightarrow> 'q1 \<Rightarrow> bool" (infix "\<in>\<^sub>1" 50)(* membership in 2/3 set *)
+    and member_2 :: "'n \<Rightarrow> 'q2 \<Rightarrow> bool" (infix "\<in>\<^sub>2" 50)(* membership in 1/3 set *)
+  assumes "\<And> q1 q2 . \<exists> q3 . \<forall> n . n \<in>\<^sub>2 q3 \<longrightarrow> n \<in>\<^sub>1 q1 \<and> n \<in>\<^sub>1 q2"  (* 2/3 quorums have 1/3 intersection *)
+    (* and "\<And> q1 q2 . \<exists> n . n \<in>\<^sub>2 q1 \<and> n \<in>\<^sub>1 q2" *) (* 2/3 sets and 1/3 sets intersect *)
+    (* and "\<And> q . \<exists> n . n \<in>\<^sub>2 q" *)
 
 record ('n,'h,'v)state =
   -- "@{typ 'n} is the type of validators (nodes), @{typ 'h} hashes, and @{typ 'v} views"
   commit_msg :: "'n \<Rightarrow> 'h \<Rightarrow> 'v \<Rightarrow> bool"
   prepare_msg :: "'n \<Rightarrow> 'h \<Rightarrow> 'v \<Rightarrow> 'v \<Rightarrow> bool"
 
-locale casper = byz_quorums + 
-  hashes:order hash_less_eq hash_less + 
+locale casper = byz_quorums +
   views:linorder view_less_eq view_less + 
-  order_bot bot for
+  order_bot  bot view_less_eq view_less for
   hash_less_eq :: "'h \<Rightarrow> 'h \<Rightarrow> bool" (infix "\<le>\<^sub>h" 50)
   and hash_less :: "'h \<Rightarrow> 'h \<Rightarrow> bool" (infix "<\<^sub>h" 50)
   and view_less_eq :: "'v \<Rightarrow> 'v \<Rightarrow> bool" (infix "\<le>\<^sub>v" 50)
   and view_less :: "'v \<Rightarrow> 'v \<Rightarrow> bool" (infix "<\<^sub>v" 50)
-  and bot::"'v" ("\<bottom>") +
-assumes "\<And> h1 h2 . \<lbrakk>h1 \<le>\<^sub>h h; h2 \<le>\<^sub>h h\<rbrakk> \<Longrightarrow> h1 \<le>\<^sub>h h2 \<or> h2 \<le>\<^sub>h h1"
-  -- "a hash has a unique parent"
+  and bot::"'v" ("\<bottom>")
 begin
 
-lemmas casper_assms = casper_axioms casper_def class.linorder_def class.order_def
+lemmas casper_assms_def = casper_def class.linorder_def class.order_def
     class.preorder_def class.order_axioms_def class.linorder_axioms_def byz_quorums_def
+    class.order_bot_def class.order_bot_axioms_def
 
-definition is_pred where "is_pred h1 h2 \<equiv> h1 <\<^sub>h h2 \<and> (\<forall> h . \<not> (h1 <\<^sub>h h \<and> h <\<^sub>h h2))"
+definition is_pred where 
+  -- "predecessor"
+  "is_pred h1 h2 \<equiv> h1 <\<^sub>h h2 \<and> (\<forall> h . \<not> (h1 <\<^sub>h h \<and> h <\<^sub>h h2))" 
+notation is_pred (infix "\<leftarrow>" 50)
+
+text {* All messages in epoch @{term \<bottom>} are ignored;  @{term \<bottom>} is used as a special value. *}
 
 definition prepared where 
-  "prepared s q h v1 v2 \<equiv> \<forall> n . member_1 n q \<longrightarrow> prepare_msg s n h v1 v2"
+  "prepared s q h v1 v2 \<equiv> v1 \<noteq> \<bottom> \<and> (\<forall> n . n \<in>\<^sub>1 q \<longrightarrow> prepare_msg s n h v1 v2)"
 definition committed where
-  "committed s q h v \<equiv> \<forall> n . member_1 n q \<longrightarrow> commit_msg s n h v"
+  "committed s q h v \<equiv> v \<noteq> bot \<and> (\<forall> n . n \<in>\<^sub>1 q \<longrightarrow> commit_msg s n h v)"
 definition fork where 
   "fork s \<equiv> \<exists> h1 h2 q1 q2 v1 v2 . committed s q1 h1 v1 \<and> committed s q2 h2 v2
     \<and> \<not>(h2 \<le>\<^sub>h h1 \<or> h1 \<le>\<^sub>h h2)"
 
 definition slashed_1 where  "slashed_1 s n \<equiv> 
-  \<exists> h v . commit_msg s n h v \<and> (\<forall> q v2 . v2 \<le>\<^sub>v v \<longrightarrow> \<not>prepared s q h v v2)"
-definition slashed_2 where "slashed_2 s n \<equiv>
+  \<exists> h v . commit_msg s n h v \<and> (\<forall> q v2 . v2 <\<^sub>v v \<longrightarrow> \<not>prepared s q h v v2)"
+definition slashed_2 where
+  "slashed_2 s n \<equiv>
   \<exists> h v1 v2 . prepare_msg s n h v1 v2 \<and> v2 \<noteq> \<bottom> \<and>
-    (\<forall> v3 q h2 . v3 \<le>\<^sub>v v2 \<longrightarrow> \<not>(prepared s q h2 v2 v3 \<and> is_pred h2 h))"
-definition slashed_3 where "slashed_3 s n \<equiv>
+    (\<forall> v3 q h2 . v3 <\<^sub>v v2 \<longrightarrow> \<not>(h2 \<leftarrow> h \<and> prepared s q h2 v2 v3))"
+definition slashed_3 where 
+  "slashed_3 s n \<equiv>
   \<exists> h1 h2 v1 v2 v3 . v1 <\<^sub>v v2 \<and> v3 <\<^sub>v v1 \<and> 
     commit_msg s n h1 v1 \<and> prepare_msg s n h2 v2 v3"
-definition slashed_4 where "slashed_4 s n \<equiv>
-  \<exists> h1 h2 v v1 v2 . (h1 \<noteq> h2 \<or> v1 \<noteq> v2) \<and> 
+definition slashed_4 where
+  "slashed_4 s n \<equiv> \<exists> h1 h2 v v1 v2 . (h1 \<noteq> h2 \<or> v1 \<noteq> v2) \<and> 
     prepare_msg s n h1 v v1 \<and> prepare_msg s n h2 v v2"
+
+definition slashed_2a where "slashed_2a s n \<equiv>
+  \<exists> h v1 . prepare_msg s n h v1 \<bottom> \<and> 
+    (\<forall> h2 q v2 . h2 \<leftarrow> h \<longrightarrow> \<not>prepared s q h2 \<bottom> v2)"
+definition slashed_5 where 
+  "slashed_5 s n \<equiv> \<exists> h v1 v2 . prepare_msg s n h v1 v2 \<and> v1 \<noteq> \<bottom> \<and> v1 \<le>\<^sub>v v2"
+
 definition slashed where "slashed s n \<equiv> 
-  slashed_1 s n \<or> slashed_2 s n \<or> slashed_3 s n \<or> slashed_4 s n"
+  slashed_1 s n \<or> slashed_2 s n \<or> slashed_3 s n \<or>  slashed_4 s n"
 
-lemma assumes "fork s" 
-  shows "\<exists> q . \<forall> n . member_2 n q \<longrightarrow> slashed s n"
-  using [[show_types]]
-  nitpick[verbose, card 'b=2, card 'c=2, card 'a=5, card 'v=2, card 'h=3, card 'd=1,
-      card "('a, 'h, 'v, 'd) state_scheme" = 1, dont_box]
-
-end
-
-end
+lemma assumes "fork s"
+  shows "\<exists> q . \<forall> n . n \<in>\<^sub>2 q \<longrightarrow> slashed s n"
+  using [[]]
+  nitpick[verbose, card 'b=2, card 'c=2, card 'a=5, card 'v=6, card 'h=5, card 'd=1,
+      card "('a, 'h, 'v, 'd) state_scheme" = 1, dont_box] (*,
+      eval="(slashed s, committed s)"] *)
+  using assms casper_axioms
+  apply -
+  unfolding slashed_def slashed_1_def slashed_2_def slashed_4_def slashed_3_def
+      prepared_def is_pred_def fork_def committed_def slashed_2a_def
+  apply (cases s)
+  apply simp
+  unfolding casper_assms_def
+  apply (simp (no_asm_use))
+  apply (match premises in P[thin]:"?x = ?y" \<Rightarrow> \<open>-\<close>)
+  apply clarify
+  using [[smt_timeout=3000,smt_oracle=true,smt_random_seed=4542,smt_certificates="./casper.cert"]]
+  sledgehammer[timeout=5000, provers=z3 spass]()
 
 
 end
